remove unused theorem again

Clean/Gadgets/Keccak/KeccakState.lean
@@ -14,37 +14,6 @@ def KeccakState.is_normalized (state : KeccakState (F p)) :=
 
 def KeccakState.value (state : KeccakState (F p)) := state.map U64.value
 
-def KeccakState.is_normalized_iff (state : KeccakState (F p)) :
-    state.is_normalized ↔
-    state[0].is_normalized ∧
-    state[1].is_normalized ∧
-    state[2].is_normalized ∧
-    state[3].is_normalized ∧
-    state[4].is_normalized ∧
-    state[5].is_normalized ∧
-    state[6].is_normalized ∧
-    state[7].is_normalized ∧
-    state[8].is_normalized ∧
-    state[9].is_normalized ∧
-    state[10].is_normalized ∧
-    state[11].is_normalized ∧
-    state[12].is_normalized ∧
-    state[13].is_normalized ∧
-    state[14].is_normalized ∧
-    state[15].is_normalized ∧
-    state[16].is_normalized ∧
-    state[17].is_normalized ∧
-    state[18].is_normalized ∧
-    state[19].is_normalized ∧
-    state[20].is_normalized ∧
-    state[21].is_normalized ∧
-    state[22].is_normalized ∧
-    state[23].is_normalized ∧
-    state[24].is_normalized := by
-  simp only [KeccakState.is_normalized, Fin.getElem_fin, Fin.forall_fin_succ, Fin.isValue,
-    Fin.val_zero, Fin.val_succ, zero_add, Nat.reduceAdd, Fin.val_eq_zero, IsEmpty.forall_iff,
-    and_true]
-
 @[reducible]
 def KeccakRow := ProvableVector U64 5
 
