Clean/Gadgets/Keccak/ThetaD.lean
@@ -57,8 +57,6 @@ theorem soundness : Soundness (F p) assumptions spec := by
     rw [←h_input, Vector.getElem_map]
 
   simp only [s] at h_holds
-  simp [circuit_norm, spec, KeccakRow.is_normalized_iff, KeccakRow.value, KeccakState.value]
-
   obtain ⟨ h_rot0, h_xor0, h_rot1, h_xor1, h_rot2, h_xor2, h_rot3, h_xor3, h_rot4, h_xor4 ⟩ := h_holds
 
   specialize h_rot0 (state_norm 1)
@@ -81,9 +79,9 @@ theorem soundness : Soundness (F p) assumptions spec := by
   specialize h_xor4 (state_norm 3) h_rot4.right
   rw [h_rot4.left] at h_xor4
 
+  simp only [circuit_norm, spec, KeccakRow.is_normalized_iff, KeccakRow.value, KeccakState.value]
   simp [Specs.Keccak256.theta_d, h_xor0, h_xor1, h_xor2, h_xor3, h_xor4, Specs.Keccak256.rol_u64, eval_vector]
   get_elem_tactic
-
 
 theorem completeness : Completeness (F p) KeccakRow assumptions := by
   intro i0 env state_var h_env state h_input h_assumptions
